ML_SP_Domain.v
@@ -5,8 +5,8 @@
 
 Set Implicit Arguments.
 Require Import Lib_FinSet Metatheory List ListSet Arith.
-Require Import ML_SP_Infrastructure ML_SP_Soundness ML_SP_Eval.
-Require Import ML_SP_Unify ML_SP_Rename ML_SP_Inference.
+Require Import ML_SP_Eval_red.
+(* Require Import ML_SP_Unify ML_SP_Rename ML_SP_Inference. *)
 
 Section ListSet.
   Variable A : Type.
@@ -161,33 +161,13 @@ Module Const.
     end.
 End Const.
 
-Module Infer := MkInfer(Cstr)(Const).
+(* Module Infer := MkInfer(Cstr)(Const).
 Import Infer.
-Import Rename.Unify.MyEval.
-(* Module MyEval := MkEval(Cstr)(Const).
-Import MyEval. *)
+Import Rename.Unify.MyEval. *)
+Module MyEval := MkEval(Cstr)(Const).
+Import MyEval.
 Import Sound.Infra.
 Import Defs.
-
-Inductive closed_n : nat -> trm -> Prop :=
-  | cln_fvar : forall n x, closed_n n (trm_fvar x)
-  | cln_bvar : forall n m, m < n -> closed_n n (trm_bvar m)
-  | cln_app  : forall n t1 t2,
-      closed_n n t1 -> closed_n n t2 -> closed_n n (trm_app t1 t2)
-  | cln_cst  : forall n c, closed_n n (trm_cst c).
-
-Lemma term_trm_inst_closed : forall t tl,
-  closed_n (length tl) t -> list_forall term tl -> term (trm_inst t tl).
-Proof.
-  unfold trm_inst; induction t; intros; inversions H; simpl; auto.
-  rewrite <- minus_n_O.
-  generalize (trm_bvar n).
-  clear H; gen tl; induction n; intros; destruct tl; try elim (lt_n_O _ H3).
-    simpl. inversion* H0.
-  simpl.
-  apply IHn. inversion* H0.
-  apply* lt_S_n.
-Qed.
 
 Module Delta.
   Definition matches_arg n := typ_arrow (typ_bvar n) (typ_bvar 1).
@@ -232,47 +212,53 @@ Module Delta.
         (Some (Kind (@valid_matches l) (coherent_matches ND)) ::
          map (fun _ => None) (seq 0 (S (length l))))
     end.
-  Definition matches_lhs l (ND:NoDup l) k :=
-    trm_app
-      (const_app (Const.matches ND) (map trm_bvar (seq 1 (length l))))
-      (trm_app (trm_cst (Const.tag (nth k l var_default)))
-        (trm_bvar 0)).
-  Definition matches_rhs k :=
-    trm_app (trm_bvar (S k)) (trm_bvar 0).
-  Definition rule n t1 t2 :=
-    exists l, exists ND:NoDup l, exists k,
-      n = S (length l) /\ k < length l /\
-      t1 = matches_lhs ND k /\ t2 = matches_rhs k.
 
-  Hint Constructors closed_n.
-  Lemma closed_n_fold_app : forall n m k t,
-    m + k <= n -> closed_n n t ->
-    closed_n n (fold_left trm_app (map trm_bvar (seq k m)) t).
+  Definition trm_default := trm_fvar var_default.
+
+  Definition reduce c tl (vl:list_for_n value (S(Const.arity c)) tl) :=
+    match c with
+    | Const.tag _ => trm_default
+    | Const.matches l nd =>
+      match nth (length l) tl trm_def with
+      | trm_app (trm_cst (Const.tag t)) t1 =>
+        match index eq_var_dec 0 t l with
+        | Some i => trm_app (nth i tl trm_def) t1
+        | None => trm_default
+        end
+      | _ => trm_default
+      end
+    end.
+
+  Lemma value_term : forall e,
+    value e -> term e.
   Proof.
-    induction m; simpl; intros.
-      auto.
-    apply IHm. omega.
-    apply* cln_app.
-    apply cln_bvar. omega.
+    intros. destruct H. induction H; auto.
   Qed.
-  Lemma term : forall n t1 t2 tl,
-    rule n t1 t2 ->
-    list_for_n term n tl ->
-    term (trm_inst t1 tl) /\ term (trm_inst t2 tl).
+
+  Lemma term : forall c tl vl,
+    term (@reduce c tl vl).
   Proof.
     intros.
-    destruct H as [l [ND [k [N [K [T1 T2]]]]]].
-    subst.
-    destruct H0.
-    split; apply* term_trm_inst_closed.
-      unfold matches_lhs.
-      apply cln_app.
-      unfold const_app.
-      apply* closed_n_fold_app. destruct H0; omega.
-      apply* cln_app.
-      apply cln_bvar. destruct H0; omega.
-    unfold matches_rhs.
-    apply cln_app; apply cln_bvar; omega.
+    case vl; clear vl; intros.
+    destruct c; simpl in *.
+      apply term_var.
+    assert (length l0 < S (length l0)) by auto.
+    rewrite e in H.
+    case_eq (nth (length l0) tl trm_def); intros; try apply term_var.
+    destruct t; try apply term_var.
+    destruct c; try apply term_var.
+    case_eq (index eq_var_dec 0 v l0); intros; try apply term_var.
+    apply term_app.
+      destruct (index_ok eq_var_dec var_default _ _ H1).
+      apply value_term.
+      apply* (list_forall_out l).
+      apply* nth_In. omega.
+    assert (term (nth (length l0) tl trm_def)).
+      apply value_term.
+      apply* (list_forall_out l).
+      apply* nth_In.
+    rewrite H0 in H2.
+    inversion* H2.
   Qed.
 
   Lemma closed : forall c, sch_fv (Delta.type c) = {}.
@@ -344,10 +330,10 @@ Module Delta.
   Qed.
 End Delta.
 
-Module Infer2 := Infer.Mk2(Delta).
-Import Infer2.Rename2.MyEval2.
-(* Module MyEval2 := Mk2(Delta).
-Import MyEval2. *)
+(* Module Infer2 := Infer.Mk2(Delta).
+Import Infer2.Rename2.MyEval2. *)
+Module MyEval2 := Mk2(Delta).
+Import MyEval2.
 Import Sound2.
 Import JudgInfra.
 Import Judge.
@@ -399,155 +385,7 @@ Module SndHyp.
     intros. rewrite H1. apply* nth_In.
   Qed.
 
-  Lemma nth_map : forall (A:Set) d1 (B:Set) (f:A->B) d2 n l,
-    n < length l -> nth n (map f l) d2 = f (nth n l d1).
-  Proof.
-    induction n; intros; destruct l; try elim (lt_n_O _ H); simpl in *.
-      auto.
-    apply IHn. apply* lt_S_n.
-  Qed.
-
-  Require Import Min.
-
   Hint Rewrite combine_length combine_nth : list.
-
-  Lemma get_kind_for_matches : forall k l (ND:NoDup l) t K E gc Us,
-    k < length l ->
-    proper_instance K (sch_kinds (Delta.type (Const.matches ND))) Us ->
-    K; E |(false,gc)|= trm_app (trm_cst (Const.tag (nth k l var_default)))
-                    t ~: nth 0 Us typ_def ->
-    K; E |(false,gc)|= t ~: nth (S (S k)) Us typ_def.
-  Proof.
-    introv Hk PI Typ.
-    destruct PI as [[Arity _] WK].
-    simpl in Arity. autorewrite with list in Arity.
-    simpl in WK.
-    destruct* Us. destruct* Us. simpl in *.
-    inversion Arity as [Ary]; clear Arity.
-    destruct WK as [WK _].
-    inversions WK. clear WK.
-    destruct H2 as [_ HE]. simpl in *.
-    inversions Typ; try discriminate. clear Typ.
-    rewrite gc_lower_false in *.
-    inversions H4; try discriminate. clear H4 H8.
-    destruct H9 as [_ WK'].
-    destruct* Us0. discriminate.
-    simpl in WK'. destruct WK' as [_ WK].
-    destruct* Us0.
-    destruct* Us0.
-    destruct WK as [WK _].
-    inversions WK. clear WK; simpl in *.
-    inversions H2; clear H2.
-    use (binds_func H0 H1). inversion H; clear H H1; subst k'0.
-    destruct H4; simpl in *.
-    destruct k' as [kc kv kr kh]; simpl in *.
-    rewrite (kh (nth k l var_default) t0 (nth k Us typ_def)) in H6; auto.
-      unfold Cstr.unique.
-      destruct H as [Hlow _]. simpl in Hlow.
-      apply set_mem_correct2.
-      apply* Hlow.
-    apply HE.
-    clear HE t0 H6 H7 H H1.
-    rewrite* <- combine_nth.
-    apply* nth_In_eq.
-        rewrite combine_length.
-        rewrite* min_l.
-        rewrite* Ary.
-      autorewrite with list.
-      rewrite* min_l.
-    rewrite* (nth_map (var_default, typ_def));
-      autorewrite with list; simpl; autorewrite with list; auto.
-      rewrite (nth_map 0).
-        rewrite* seq_nth.
-      rewrite* seq_length.
-    rewrite* min_l.
-  Qed.
-
-  Lemma delta_typed : forall n t1 t2 tl K E gc T,
-    Delta.rule n t1 t2 ->
-    list_for_n term n tl ->
-    K ; E |(false,gc)|= trm_inst t1 tl ~: T ->
-    K ; E |(false,gc)|= trm_inst t2 tl ~: T.
-  Proof.
-    intros.
-    clear H0.
-    destruct H as [l [ND [k [HN [HK [T1 T2]]]]]].
-    subst.
-    inversions H1; try discriminate; clear H1.
-    rewrite gc_lower_false in *.
-    rewrite trm_inst_app in H4.
-    unfold const_app in H4.
-    destruct (fold_app_inv _ _ H4) as [TL [Typ0 TypA]]; clear H4.
-    unfold trm_inst; simpl.
-    inversions Typ0; try discriminate. clear Typ0 H1 H4.
-    unfold sch_open in H0. simpl in H0.
-    destruct (fold_arrow_eq _ _ _ _ _ H0); clear H0.
-      generalize (For_all2_length _ _ _ TypA).
-      autorewrite with list. auto.
-    generalize (For_all2_nth _ trm_def typ_def _ TL TypA (n:=k)); clear TypA.
-    autorewrite with list; intro TypA.
-    generalize (For_all2_nth _ typ_def typ_def _ TL H1 (n:=k)); clear H1.
-    autorewrite with list; intro EQ.
-    rewrite <- EQ in TypA; auto; clear EQ TL.
-    rewrite (map_nth trm_def trm_def) in TypA.
-     rewrite (map_nth trm_def 0) in TypA.
-      rewrite seq_nth in TypA; auto.
-      rewrite (map_nth typ_def 0) in TypA.
-       rewrite seq_nth in TypA; auto.
-       simpl in TypA, H.
-       inversions H; clear H.
-       eapply typing_app; rewrite* gc_lower_false.
-       apply* get_kind_for_matches.
-      rewrite* seq_length.
-     rewrite* seq_length.
-    autorewrite with list; auto.
-  Qed.
-
-  Fixpoint typ_arity (T:typ) : nat :=
-    match T with
-    | typ_arrow T1 T2 => S (typ_arity T2)
-    | _ => 0
-    end.
-
-  Lemma fold_arrow_open : forall T TL Us,
-    typ_open (fold_right typ_arrow T TL) Us =
-    fold_right typ_arrow (typ_open T Us) (map (fun T:typ => typ_open T Us) TL).
-  Proof.
-    induction TL; simpl; intros; auto.
-    rewrite* IHTL.
-  Qed.
-
-  Lemma typ_arity_fold_arrow : forall T TL,
-    typ_arity (fold_right typ_arrow T TL) = length TL + typ_arity T.
-  Proof.
-    induction TL; simpl; auto.
-  Qed.
-
-  Lemma value_is_tag : forall K gc v n T,
-    K; empty |(false,gc)|= v ~: T ->
-    valu n v ->
-    typ_arity T <= n ->
-    exists l, exists tl, v = const_app (Const.tag l) tl.
-  Proof.
-    induction v; introv Typv Hv TA; inversions Hv; inversions Typv;
-      try discriminate.
-      simpl in TA. elim (le_Sn_O _ TA).
-      clear IHv2.
-      rewrite gc_lower_false in *.
-      destruct* (IHv1 (Datatypes.S n) _ H5) as [l [tl EQ]].
-        simpl. apply* le_n_S.
-      exists l. exists (tl ++ v2 :: nil).
-      rewrite EQ.
-      unfold const_app; rewrite fold_left_app. auto.
-    destruct c.
-      exists v. exists (nil (A:=trm)). auto.
-    elim (le_not_lt _ _ TA). clear.
-    unfold sch_open; simpl.
-    rewrite fold_arrow_open.
-    rewrite typ_arity_fold_arrow.
-    autorewrite with list.
-    simpl. omega.
-  Qed.
 
   Lemma tag_is_const : forall v vl K E gc T TL,
     S (Const.arity (Const.tag v)) = length vl ->
@@ -571,202 +409,222 @@ Module SndHyp.
     discriminate.
   Qed.
 
-  Lemma seq_in : forall k n m, In k (seq m n) -> m <= k < m+n.
-  Proof.
-    induction n; intros. elim H.
-    simpl in H; destruct H.
-      rewrite H. omega.
-    destruct* (IHn (S m)).
-    omega.
-  Qed.
-
-  Lemma map_inst_bvar : forall t l,
-    l = map (trm_inst_rec 0 (t :: l)) (map trm_bvar (seq 1 (length l))).
-  Proof.
-    induction l; simpl; auto.
-    apply (f_equal (cons a)).
-    rewrite <- seq_shift.
-    pattern l at 1. rewrite IHl.
-    clear.
-    rewrite map_map.
-    rewrite map_map.
-    rewrite map_map.
-    apply list_map_ext.
-    intros.
-    simpl.
-    rewrite <- minus_n_O.
-    destruct (seq_in _ _ _ H).
-    destruct x.
-      elim (le_Sn_O _ H0).
-    apply nth_indep. omega.
-  Qed.
-
-  Lemma typing_tag_inv : forall K E gc l tl x,
-    K; E |(false,gc)|= const_app (Const.tag l) tl ~: typ_fvar x ->
-    exists t, exists T, exists k,
-      tl = t :: nil /\  K; E |(false,gc)|= t ~: T /\ binds x (Some k) K
-      /\ exists M, entails k (@Kind _ (Delta.valid_tag l) ((l, T) :: nil) M).
-  Proof.
-    introv Typv.
-    unfold const_app in Typv.
-    destruct* (fold_app_inv _ _ Typv) as [TL [Typc Typa]]; clear Typv.
-    inversions Typc; try discriminate. clear Typc H1 H4.
-    destruct H5 as [_ WK].
-    unfold sch_open in H0; simpl in H0.
-    destruct TL as [|T TL]. discriminate.
-    destruct tl. elim Typa.
-    exists t. exists T.
-    simpl in H0; inversions H0; clear H0.
-    simpl in WK.
-    destruct* Us. destruct* Us. destruct* Us.
-    destruct WK as [_ [WK _]].
-    inversions WK; clear WK.
-    exists k'.
-    destruct TL; try discriminate.
-    simpl in H2; inversion H2; subst x0; clear H2.
-    simpl in Typa.
-    destruct Typa.
-    destruct tl; try elim H1.
-    intuition.
-    unfold ckind_map in H3.
-    destruct (ckind_map_spec
-               (fun T : typ => typ_open T (t0 :: typ_fvar x :: nil))
-               (Kind (Delta.valid_tag l) (Delta.coherent_tag (t:=l)))).
-    destruct x0 as [kc kv kr kh]; simpl in *.
-    destruct a; subst.
-    exists* kh.
-  Qed.
-
-  Lemma const_arity_ok0 : forall c vl K E gc T,
-    S(Const.arity c) = length vl ->
-    K ; E |(false,gc)|= const_app c vl ~: T ->
-    exists l, exists ND : NoDup l, exists Us, exists v, exists vl',
-      vl = rev (v :: vl') /\ c = Const.matches ND /\ length l = length vl' /\
-      proper_instance K (sch_kinds (Delta.type (Const.matches ND))) Us /\
-      K; E |(false,gc)|= v ~: nth 0 Us typ_def.
+  Lemma matches_not_value : forall K E gc i x TL t,
+    K;E |(false,gc)|= t ~: fold_right typ_arrow (typ_fvar x) TL ->
+    valu (length TL + i) t ->
+    length TL <= 1.
   Proof.
     intros.
-    unfold const_app in H0.
-    use (fold_app_inv _ _ H0).
-    clear H0; destruct H1 as [TL [TypC TypA]].
-    destruct c.
-      elim (tag_is_const _ _ _ H TypC TypA).
-    exists l. exists n.
-    inversions TypC; try discriminate. clear TypC H5.
-    exists Us.
-    simpl in H.
-    unfold sch_open in H1; simpl in H1.
-    rewrite <- (rev_involutive TL) in *.
-    destruct (rev TL) as [|T' TL'].
-      destruct vl. discriminate.
-      elim TypA.
-    rewrite <- (rev_involutive vl) in *.
-    destruct (rev vl) as [|v vl'].
-      discriminate.
-    exists v. exists vl'.
-    rewrite rev_length in H. simpl in H; inversion* H.
-    intuition.
-    use (For_all2_rev _ _ _ TypA); clear TypA.
-    autorewrite with list in H0.
-    simpl in H0; destruct H0 as [Typv TypA].
-    rewrite cons_append in H1.
-    rewrite distr_rev in H1.
-    rewrite fold_right_app in H1. simpl in H1.
-    destruct (fold_arrow_eq _ _ _ _ _ H1); clear H1.
-      autorewrite with list.
-      rewrite H3. apply* For_all2_length.
-    simpl in H0. inversions* H0.
+    gen_eq (length TL + i) as j.
+    gen TL; induction H0; intros; subst; try discriminate.
+        omega.
+      destruct c; simpl in *.
+        omega.
+      inversions H; clear H; try discriminate.
+      unfold sch_open in H2; simpl in *.
+      rewrite H1 in H2.
+      simpl in H2.
+      clear -H2.
+      elimtype False.
+      revert H2; generalize 2; induction TL; simpl; intros.
+        destruct i; discriminate.
+      inversions* H2.
+    inversions H; clear H; try discriminate.
+    rewrite gc_lower_false in *.
+    forward~ (IHvalu1 (S::TL)) as IH.
+    simpl in IH. omega.
   Qed.
 
-  Lemma const_arity_ok : forall c vl K gc T,
-    list_for_n value (S(Const.arity c)) vl ->
-    K ; empty |(false,gc)|= const_app c vl ~: T ->
-    exists n:nat, exists t1:trm, exists t2:trm, exists tl:list trm,
-      Delta.rule n t1 t2 /\ list_for_n term n tl /\
-      const_app c vl = trm_inst t1 tl.
+  Lemma value_fvar_is_const : forall K E gc t x,
+    K; E |(false,gc)|= t ~: typ_fvar x ->
+    value t ->
+    exists v, exists t2, t = trm_app (trm_cst (Const.tag v)) t2.
   Proof.
     intros.
-    destruct (const_arity_ok0 _ _ (proj1 H) H0) as
-      [l [ND [Us [v [vl' [Evl [Ec [Hvl' [PI Typv]]]]]]]]]; clear H0.
-    subst.
-    exists (S (length l)).
-    destruct PI as [_ WK].
-    destruct Us; simpl in Typv.
-      assert (type typ_def). auto.
-      inversion H0.
-    destruct H as [_ Val].
-    use (list_forall_rev Val); clear Val.
-    rewrite rev_involutive in H.
-    inversions H; clear H.
-    destruct H3 as [vn Hv].
-    use (proj1 WK). inversions H; clear H WK.
-    destruct* (value_is_tag (n:=vn) Typv) as [l' [tl' EQ]].
-      auto with arith.
-    clear vn Hv.
-    subst.
-    destruct (typing_tag_inv _ _ Typv) as
-      [t [T' [k [EQ [Typa [Bk Ek]]]]]]; clear Typv.
-    use (binds_func H1 Bk). inversion H; subst; clear H H1.
-    destruct H4 as [[_ High] _].
-    destruct Ek as [M [[Low _] _]].
-    destruct k as [[kl kh] kv kr kch]; simpl in *.
-    destruct* kh as [kh|].
-    unfold Cstr.valid in kv. simpl in kv.
-    assert (In l' l) by auto.
-    clear High Low kl kh kv kr kch Bk x Us.
-    destruct (exists_nth var_default _ _ H) as [n [Hlen EQ]].
-    clear H; subst l'.
-    exists (Delta.matches_lhs ND n).
-    exists (Delta.matches_rhs n).
-    exists (t :: rev vl').
-    split3.
-      unfold Delta.rule. exists l; exists ND; exists n. auto.
-      split*. simpl. rewrite rev_length. rewrite* Hvl'.
-      constructor; auto.
-      apply* list_forall_rev.
-      apply (list_forall_imp _ value_regular H2).
-    unfold Delta.matches_lhs.
-    unfold trm_inst.
-    simpl; rewrite trm_inst_app.
-    unfold const_app.
-    rewrite fold_left_app.
-    simpl.
-    rewrite Hvl'.
-    rewrite <- (rev_length vl').
-    rewrite <- (map_inst_bvar t (rev vl')).
-    auto.
+    destruct H0 as [i vi].
+    inversions vi; clear vi.
+        inversion H; discriminate.
+      destruct c; inversions H; try discriminate.
+      unfold sch_open in *; simpl in *.
+      clear -H1.
+      destruct (length l); discriminate.
+    inversions H; clear H; try discriminate.
+    rewrite gc_lower_false in *.
+    inversions H0; clear H0.
+      destruct c; inversions H6; clear H6; try discriminate.
+        esplit; esplit; reflexivity.
+      simpl in H2.
+      unfold sch_open in *; simpl in *.
+      rewrite H2 in H0. simpl in H0.
+      inversions H0.
+      destruct i; discriminate.
+    inversions H6; clear H6; try discriminate. rewrite gc_lower_false in *.
+    puts (matches_not_value i x (S0 :: S :: nil) H7 H).
+    elimtype False. simpl in H0. omega.
+  Qed.
+
+  Lemma fold_right_app_end : forall T1 T2 TL,
+    fold_right typ_arrow (typ_arrow T1 T2) TL =
+    fold_right typ_arrow T2 (TL ++ T1 :: nil).
+  Proof.
+    intros; rewrite* fold_right_app.
   Qed.
     
-  Lemma delta_arity : forall n t1 t2,
-    Delta.rule n t1 t2 ->
-    exists c, exists pl, t1 = const_app c pl /\ length pl = S(Const.arity c).
+
+  Lemma delta_matches : forall l n tl K E gc T,
+    list_for_n value (S (Const.arity (@Const.matches l n))) tl ->
+    K ; E |(false,gc)|= const_app (Const.matches n) tl ~: T ->
+    exists v, exists t, In v l /\
+      nth (length l) tl trm_def = trm_app (trm_cst (Const.tag v)) t.
   Proof.
     intros.
-    destruct H as [tl [ND [k [L1 [L2 [LHS RHS]]]]]].
-    unfold Delta.matches_lhs in LHS.
-    exists (Const.matches ND).
-    exists (map trm_bvar (seq 1 (length tl)) ++
-            trm_app (trm_cst (Const.tag (nth k tl var_default))) (trm_bvar 0)
-            :: nil).
-    split.
-      rewrite LHS.
-      unfold const_app.
-      rewrite fold_left_app.
-      simpl. auto.
+    destruct (fold_app_inv _ _ H0) as [TL [Typ0 TypA]]; clear H0.
+    inversions Typ0; try discriminate. clear Typ0.
+    unfold sch_open in H1. simpl in H1.
+    rewrite fold_right_app_end in H1.
+    destruct H as [Hlen Htl]. simpl in Hlen.
+    destruct (fold_arrow_eq _ _ _ _ _ H1); clear H1.
+      generalize (For_all2_length _ _ _ TypA).
+      autorewrite with list. simpl. intros; omega.
+    forward~ (For_all2_nth _ trm_def typ_def _ TL TypA (n:=length l)) as Typn.
+      rewrite* <- Hlen.
+    forward~ (For_all2_nth _ typ_def typ_def _ TL H0 (n:=length l)) as Typn'.
+      autorewrite with list. simpl*. omega.
+    rewrite app_nth2 in Typn'; autorewrite with list in Typn' |- *; auto.
+    rewrite <- minus_n_n in Typn'.
+    simpl in Typn'.
+    puts (proj2 H6). simpl in H1.
+    do 2 destruct* Us.
+    simpl in Typn'.
+    destruct H1 as [Ht [_ HUs]].
+    inversions Ht; clear Ht.
+    rewrite <- H8 in *.
+    destruct (value_fvar_is_const Typn) as [v [t2 Hv]].
+      apply* (list_forall_out Htl). apply* nth_In. omega.
     simpl.
-    autorewrite with list.
-    simpl.
-    rewrite plus_comm.
-    auto.
+    rewrite Hv in *.
+    inversions Typn; clear Typn; try discriminate.
+    rewrite gc_lower_false in *.
+    inversions H10; clear H10; try discriminate.
+    destruct H15.
+    destruct H. simpl in H.
+    do 3 (destruct Us0; try discriminate).
+    simpl in *.
+    destruct H1 as [_ [Ht1 _]].
+    subst t1.
+    inversions Ht1; clear Ht1.
+    puts (binds_func H11 H3).
+    inversions H1; clear H H1 H11.
+    destruct H15; destruct H7. simpl in *.
+    destruct H; destruct H4. simpl in *. clear H10.
+    destruct k' as [[kcl kch] kv kr kh]; simpl in *.
+    assert (Hvt: In (v,t) kr) by auto*. clear H1.
+    destruct* kch.
+    unfold Cstr.valid in kv; simpl in kv.
+    assert (In v l) by auto*.
+    exists v. exists t2.
+    split*.
+Qed.
+
+  Lemma delta_typed : forall c tl vl K E gc T,
+    K ; E |(false,gc)|= const_app c tl ~: T ->
+    K ; E |(false,gc)|= @Delta.reduce c tl vl ~: T.
+  Proof.
+    intros.
+    destruct (fold_app_inv _ _ H) as [TL [Typ0 TypA]]; clear H.
+    destruct c.
+      elim (tag_is_const _ _ _ (proj1 vl) Typ0 TypA).
+    inversions Typ0; try discriminate. clear Typ0.
+    unfold sch_open in H0. simpl in H0.
+    assert (forall T1 T2 TL, fold_right typ_arrow (typ_arrow T1 T2) TL =
+      fold_right typ_arrow T2 (TL ++ T1 :: nil)).
+      intros; rewrite* fold_right_app.
+    rewrite H in H0; clear H.
+    poses Hlen (proj1 vl). simpl in Hlen.
+    destruct (fold_arrow_eq _ _ _ _ _ H0); clear H0.
+      generalize (For_all2_length _ _ _ TypA).
+      autorewrite with list. simpl. intros; omega.
+    forward~ (For_all2_nth _ trm_def typ_def _ TL TypA (n:=length l)) as Typn.
+      rewrite* <- Hlen.
+    forward~ (For_all2_nth _ typ_def typ_def _ TL H2 (n:=length l)) as Typn'.
+      autorewrite with list. simpl*. omega.
+    rewrite app_nth2 in Typn'.
+      autorewrite with list in Typn'. rewrite <- minus_n_n in Typn'.
+      simpl in Typn'.
+      puts (proj2 H5). simpl in H0. destruct* Us.
+      destruct* Us.
+      simpl in Typn'.
+      destruct H0.
+      destruct H3.
+      inversions H0; clear H0.
+      rewrite <- H11 in *.
+      destruct (value_fvar_is_const Typn) as [v [t2 Hv]].
+        apply* (list_forall_out (proj2 vl)). apply* nth_In. omega.
+      simpl.
+      rewrite Hv in *.
+      inversions Typn; clear Typn; try discriminate.
+      rewrite gc_lower_false in *.
+      inversions H12; clear H12; try discriminate.
+      destruct H17.
+      destruct H. simpl in H.
+      do 3 (destruct Us0; try discriminate).
+      simpl in *.
+      destruct H0 as [_ [Ht1 _]].
+      subst t1.
+      inversions Ht1; clear Ht1.
+      puts (binds_func H13 H8).
+      inversions H0; clear H0 H13.
+      destruct H17; destruct H10. simpl in *.
+      destruct H0; destruct H10. simpl in *.
+      destruct k' as [[kcl kch] kv kr kh]; simpl in *.
+      assert (Hvt: In (v,t) kr) by auto*. clear H7 H13.
+      destruct* kch.
+      unfold Cstr.valid in kv; simpl in kv.
+      assert (In v l) by auto*.
+      case_eq (index eq_var_dec 0 v l); introv R2;
+        try elim (index_none_notin _ _ _ _ R2 H7).
+      destruct (index_ok _ var_default _ _ R2).
+      forward~ (For_all2_nth _ trm_def typ_def _ TL TypA (n:=n0)) as Typv.
+        omega.
+      forward~ (For_all2_nth _ typ_def typ_def _ TL H2 (n:=n0)) as Eqv.
+        rewrite (For_all2_length _ _ _ H2).
+        rewrite <- (For_all2_length _ _ _ TypA).
+        omega.
+      rewrite app_nth1 in Eqv; [|rewrite map_length; rewrite* seq_length].
+      rewrite (map_nth _ 0) in Eqv; [|rewrite* seq_length].
+      rewrite seq_nth in Eqv; auto.
+      simpl in Eqv.
+      assert (In (v, nth n0 Us typ_def) kr).
+        rewrite <- H18.
+        apply H12.
+        clear -H13.
+        remember (0 + n0) as m.
+        pattern n0 at 2.
+        replace n0 with (0+n0) by reflexivity. rewrite <- Heqm.
+        gen n0; generalize 0; induction l; intros.
+          simpl in H13; elimtype False; omega.
+        destruct n0; simpl.
+          replace m with n; auto. omega.
+        right. apply (IHl (S n) n0).
+          simpl in H13. omega.
+        omega.
+      assert (Cstr.unique (Cstr.C kcl (Some l0)) v = true).
+        unfold Cstr.unique.
+        apply set_mem_correct2. simpl. unfold set_In. auto*.
+      puts (kh _ _ _ H20 Hvt H19).
+      rewrite <- H21 in *.
+      rewrite <- Eqv in Typv.
+      apply* typing_app; rewrite gc_lower_false; auto*.
+    rewrite map_length; rewrite seq_length; auto.
   Qed.
- 
+
   Definition get_tag cl :=
     match cl with
     | clos_const (Const.tag t) (cl1 :: nil) => Some (t, cl1)
     | _ => None
     end.
 
-  Definition delta_red c (cl : list clos) :=
+  Definition reduce_clos c (cl : list clos) :=
     match c with
     | Const.tag _ => (clos_def, nil)
     | Const.matches l nd =>
@@ -780,189 +638,68 @@ Module SndHyp.
       end
     end.
 
-  Lemma delta_red_sound : forall c cls,
-    list_for_n clos_ok (S(Const.arity c)) cls ->
-    exists t1:trm, exists t2:trm, exists tl:list trm,
-    forall K E T,
-      K ; E |Gc|= const_app c (List.map clos2trm cls) ~: T ->
-      let (cl', cls') := delta_red c cls in
-      Delta.rule (length tl) t1 t2 /\ list_forall term tl /\
-      const_app c (List.map clos2trm cls) = trm_inst t1 tl /\
-      fold_left trm_app (List.map clos2trm cls') (clos2trm cl')
-      = trm_inst t2 tl /\
-      clos_ok cl' /\ list_forall clos_ok cls'.
+  Lemma reduce_clos_sound :
+    forall c cls (CLS : list_for_n clos_ok (S(Const.arity c)) cls) K E T,
+      K; E |Gc|= const_app c (List.map clos2trm cls) ~: T ->
+      let (cl', cls') := reduce_clos c cls in
+      clos_ok cl' /\ list_forall clos_ok cls' /\
+      fold_left trm_app (List.map clos2trm cls') (clos2trm cl') =
+      Delta.reduce c (list_for_n_value CLS).
   Proof.
     intros.
+    puts (proj1 CLS).
     destruct c.
-      exists trm_def; exists trm_def; exists (@nil trm).
-      intros.
-      unfold const_app in H0.
-      puts (fold_app_inv _ _ H0).
-      clear H0; destruct H1 as [TL [TypC TypA]].
-      destruct H. rewrite <- (map_length clos2trm) in H.
-      elim (tag_is_const _ _ _ H TypC TypA).
-    unfold delta_red.
-    case_eq (get_tag (nth (length l) cls clos_def)); introv R.
-      destruct p.
-      case_eq (index eq_var_dec 0 v l); introv R1.
-        rename n0 into i.
-        exists (Delta.matches_lhs n i).
-        exists (Delta.matches_rhs i).
-        case_eq (cut (length l) cls); introv R2.
-        exists (map clos2trm (c :: l0)).
-        intros.
-        destruct H as [Hl Hcls].
-        assert (Hl': length l <= length cls).
-          simpl in Hl. rewrite <- Hl. omega.
-        destruct (cut_ok _ Hl' R2) as [Hl0 Hcut].
-        destruct (index_ok _ var_default v l R1) as [Hi Hi'].
-        destruct l1.
-          elimtype False; subst. simpl in *.
-          rewrite app_length in Hl; rewrite Hl0 in Hl.
-          simpl in Hl; omega.
-        destruct l1.
-        assert (HR: c0 = clos_const (Const.tag v) (c :: nil)).
-          unfold get_tag in R.
-          case_rewrite R3 (nth (length l) cls clos_def).
-          rewrite Hcut in R3.
-          rewrite app_nth2 in R3.
-          rewrite Hl0 in R3.
-          rewrite <- minus_n_n in R3. simpl in R3.
-          subst; simpl.
-          case_rewrite R4 c1.
-          case_rewrite R5 l1.
-          destruct l2; try discriminate.
-          inversions* R.
-          omega.
-        split.
-          rewrite map_length.
-          unfold Delta.rule.
-          simpl. exists l. exists n. exists i.
-          rewrite* Hl0.
-        split.
-          apply* (@list_forall_map _ clos_ok _ term clos2trm).
-            intros; apply* clos_ok_term.
-          rewrite Hcut in Hcls.
-          constructor.
-            apply list_forall_in; intros; apply* (list_forall_out Hcls).
-          assert (clos_ok c0) by apply* (list_forall_out Hcls).
-          rewrite HR in H; inversion H. inversion* H3.
-        split.
-          unfold Delta.matches_lhs, trm_inst; simpl.
-          rewrite trm_inst_app.
-          rewrite Hcut.
-          unfold const_app; rewrite map_app; rewrite fold_left_app.
-          simpl; apply f_equal2.
-            apply* (f_equal2 (fold_left trm_app)).
-            rewrite <- Hl0.
-            clear.
-            rewrite <- (map_length clos2trm l0).
-            apply map_inst_bvar.
-          rewrite HR.
-          rewrite Hi'.
-          reflexivity.
-        split.
-          unfold Delta.matches_rhs.
-          unfold trm_inst; simpl.
-          rewrite <- Hl0 in Hi.
-          apply* f_equal2.
-          rewrite Hcut.
-          rewrite* app_nth1.
-          symmetry; apply* map_nth.
-        split.
-          apply* (list_forall_out Hcls).
-          apply* nth_In. omega.
-        constructor; auto.
-        assert (clos_ok c0).
-          apply* (list_forall_out Hcls).
-          rewrite* Hcut.
-        rewrite HR in H; inversion H. inversion* H3.
-      elimtype False. rewrite Hcut in Hl.
-      rewrite app_length in Hl. simpl in Hl; omega.
-    exists trm_def. exists trm_def. exists (@nil trm).
-    intros; elim (index_none_notin _ _ _ _ R1); clear R1.
-    destruct H. rewrite <- (map_length clos2trm) in H.
-    destruct (const_arity_ok0 _ _ H H0)
-      as [l' [ND [Us [v' [vl' [Hcls [Hn [Hl' [PI Typ]]]]]]]]].
-    inversions Hn; clear Hn.
-    set (cl1 := nth (length l') cls clos_def) in *.
-    assert (v' = clos2trm cl1).
-      unfold cl1; rewrite <- List.map_nth.
-      rewrite Hcls.
-      rewrite rev_nth.
-      simpl. rewrite Hl'; rewrite* <- minus_n_n.
-      simpl; rewrite Hl'; auto with arith.
-    destruct cl1; try discriminate.
-    destruct c0; try discriminate.
-    destruct l; try discriminate.
-    destruct l; try discriminate.
-    inversions R.
-    destruct PI.
-    simpl in H3.
-    destruct Us; try contradiction.
-    destruct H3.
-    destruct Us; try contradiction.
-    inversions H3.
-    simpl in Typ.
-    destruct (typing_tag_inv _ _ Typ) as [t [T' [k'' [Ht [Typ' [B [M HE]]]]]]].
-    inversions Ht; clear Ht.
-    puts (binds_func B H6). inversions H5; clear H5 H6.
-    destruct HE as [[HE _] _]. simpl in HE.
-    destruct H8 as [[_ H8] _]. simpl in *.
-    destruct k' as [[kl kh] kv kr kt].
-    simpl in *.
-    unfold Cstr.valid in kv.
-    simpl in kv.
-    destruct kh; try contradiction.
-    auto*.
-  exists trm_def. exists trm_def. exists (@nil trm).
-  intros; elimtype False.
-  destruct H. rewrite <- (map_length clos2trm) in H.
-  destruct (const_arity_ok0 _ _ H H0)
-    as [l' [ND [Us [v' [vl' [Hcls [Hn [Hl' [PI Typ]]]]]]]]].
-  inversions Hn; clear Hn.
-  set (cl1 := nth (length l') cls clos_def) in *.
-  assert (v' = clos2trm cl1).
-    unfold cl1; rewrite <- List.map_nth.
-    rewrite Hcls.
-    rewrite rev_nth.
-    simpl. rewrite Hl'; rewrite* <- minus_n_n.
-    simpl; rewrite Hl'; auto with arith.
-  destruct PI.
-  simpl in H4.
-  destruct Us; try contradiction.
-  destruct H4.
-  destruct Us; try contradiction.
-  inversions H4.
-  simpl in Typ.
-  case_rewrite R1 cl1; subst; simpl in *.
-    unfold trm_inst in Typ. inversion Typ; discriminate.
-  assert (clos_ok (clos_const c l)).
-    rewrite <- R1.
-    apply (list_forall_out H1).
-    apply* nth_In. rewrite map_length in H; omega.
-  destruct c.
-    destruct (typing_tag_inv _ _ Typ) as [t [T' [k'' [Ht [Typ' [B [M HE]]]]]]].
-    destruct l; try discriminate.
-    destruct l; try discriminate.
-  inversions H2.
-  unfold const_app in Typ.
-  destruct (fold_app_inv _ _ Typ) as [TL [TypC TypA]].
-  inversions TypC; try discriminate.
-  simpl in *.
-  puts (For_all2_length _ _ _ TypA).
-  rewrite map_length in H6.
-  rewrite H6 in H11.
-  unfold sch_open in H8; simpl in H8.
-  clear -H8 H11.
-  gen l0; generalize 2; induction TL; destruct l0; intros; try discriminate.
-    simpl in H11; omega.
-  simpl in *.
-  inversions H8.
-  elim (IHTL (S n) l0). simpl in H11; omega. auto.
-Qed.
+      simpl in H0.
+      do 3 (destruct cls; try discriminate).
+      unfold const_app in H; simpl in H.
+      inversions H; try discriminate. simpl in H5.
+      inversions H5; try discriminate. simpl in H6.
+      inversions H6; try discriminate.
+      destruct H12.
+      destruct H1. simpl in H1.
+      do 3 (destruct Us; try discriminate). simpl in *.
+      destruct H2 as [_ [Ht0 _]].
+      subst. inversion Ht0.
+    destruct (delta_matches n (list_for_n_value CLS) H) as [v [t [Hv Ht]]].
+    simpl in * |-. simpl reduce_clos.
+    rewrite (map_nth _ clos_def) in Ht; try omega.
+    case_rewrite R3 (nth (length l) cls clos_def).
+    simpl in Ht. unfold const_app in Ht.
+    destruct l0; try discriminate.
+    simpl in Ht.
+    destruct l0 using rev_ind.
+      simpl in Ht; inversion Ht; clear Ht. subst.
+      simpl.
+      case_eq (index eq_var_dec 0 v l); introv R1;
+        try elim (index_none_notin _ _ _ _ R1 Hv).
+      destruct (index_ok _ var_default _ _ R1).
+      rename n0 into i.
+      assert (clos_ok (nth i cls clos_def)).
+        apply (list_forall_out (proj2 CLS)).
+        apply* nth_In.
+        omega.
+      split*.
+      assert (Htag: clos_ok (nth (length l) cls clos_def)).
+        apply (list_forall_out (proj2 CLS)).
+        apply* nth_In. omega.
+      rewrite R3 in Htag.
+      split.
+        inversion* Htag.
+      rewrite (map_nth _ clos_def); try omega.
+      rewrite R3. simpl.
+      rewrite R1.
+      rewrite (map_nth _ clos_def); auto. omega.
+    clear IHl0.
+    elimtype False.
+    rewrite map_app in Ht; rewrite fold_left_app in Ht.
+    simpl in Ht.
+    inversions Ht.
+    clear -H2; destruct l0 using rev_ind. discriminate.
+    rewrite map_app in H2; rewrite fold_left_app in H2.
+    discriminate.
+  Qed.
 End SndHyp.
 
-Module Sound3 := Infer2.Rename2.MyEval2.Mk3(SndHyp).
-(* Module Sound3 := MyEval2.Mk3(SndHyp). *)
+(* Module Sound3 := Infer2.Rename2.MyEval2.Mk3(SndHyp). *)
+Module Sound3 := MyEval2.Mk3(SndHyp).
 
